Update case study with latest changes #164

example/CaseStudyHuttonsRazor/Extra/FreeDB.v
@@ -4,15 +4,24 @@
 
 From Base Require Import Free Free.Instance.Maybe Prelude.
 From Generated Require Import Razor.
+Import AppendAssoc.
 
 Require Import Coq.Logic.FunctionalExtensionality.
 
-Arguments Nil {Shape} {Pos} {A}.
-Arguments Cons {Shape} {Pos} {A}.
-Arguments Val {Shape} {Pos}.
-Arguments Add0 {Shape} {Pos}.
-Arguments PUSH {Shape} {Pos}.
-Arguments ADD {Shape} {Pos}.
+Notation "'Nil_'" := (Nil _ _)
+  (at level 9).
+Notation "'Cons_' fx fxs" := (Cons _ _ fx fxs)
+  (at level 10, fx, fxs at level 9).
+Notation "'Val_' fn":= (Val _ _ fn)
+  (at level 10, fn at level 9).
+Notation "'Add0_' fx fy":= (Add0 _ _ fx fy)
+  (at level 10, fx, fy at level 9).
+Notation "'PUSH_' fv":= (PUSH _ _ fv)
+  (at level 10, fv at level 9).
+Notation "'ADD_'":= (ADD _ _)
+  (at level 9).
+Arguments Just {Shape'} {Pos'} {H} {A}.
+Arguments Nothing {Shape'} {Pos'} {H} {A}.
 Arguments append {Shape} {Pos} {a}.
 Arguments addInteger {Shape} {Pos}.
 Arguments eval {Shape} {Pos}.
@@ -23,120 +32,16 @@ Arguments comp' {Shape} {Pos}.
 
 (* Database for general rewriting rules to make the goal look pretty. *)
 Create HintDb prettyDB.
-(* Databases for using / unfolding smart constructors. *)
-Create HintDb smartConstrDB.
-Create HintDb invSmartConstrDB.
 (* Database with function rules. *)
 Create HintDb simplDB.
 
 (* Make the goal look pretty without changing anything. *)
 Ltac pretty :=
-  autorewrite with prettyDB smartConstrDB.
+  autorewrite with prettyDB.
 (* Try to apply function rules and solve the goal while keeping it pretty. *)
 Ltac autodef :=
-  autorewrite with invSmartConstrDB;
   autorewrite with simplDB;
-  pretty; try reflexivity.
-
-(* Define rules for rewriting smart constructors. *)
-Section Rewrite_Constructors.
-
-  Variable Shape : Type.
-  Variable Pos : Shape -> Type.
-
-  Lemma def_Nil :
-    forall (A : Type),
-        pure (@nil Shape Pos A) = Nil.
-  Proof.
-    reflexivity.
-  Qed.
-
-  Lemma def_Cons :
-    forall (A : Type)
-           (fhead : Free Shape Pos A)
-           (ftail : Free Shape Pos (List Shape Pos A)),
-        pure (cons fhead ftail) = Cons fhead ftail.
-  Proof.
-    reflexivity.
-  Qed.
-
-  Lemma def_Code_Nil :
-        pure (nil : Code Shape Pos) = Nil.
-  Proof.
-    reflexivity.
-  Qed.
-
-  Lemma def_Code_Cons :
-    forall (fhead : Free Shape Pos (Op Shape Pos))
-           (ftail : Free Shape Pos (Code Shape Pos)),
-        pure (cons fhead ftail) = Cons fhead ftail.
-  Proof.
-    reflexivity.
-  Qed.
-
-  Lemma def_Stack_Nil :
-        pure (nil : Stack Shape Pos) = Nil.
-  Proof.
-    reflexivity.
-  Qed.
-
-  Lemma def_Stack_Cons :
-    forall (fhead : Free Shape Pos (Integer Shape Pos))
-           (ftail : Free Shape Pos (Stack Shape Pos)),
-        pure (cons fhead ftail) = Cons fhead ftail.
-  Proof.
-    reflexivity.
-  Qed.
-
-  Lemma def_Val :
-    forall (fn : Free Shape Pos (Integer Shape Pos)),
-        pure (val fn) = Val fn.
-  Proof.
-    reflexivity.
-  Qed.
-
-  Lemma def_Add :
-    forall (fx fy : Free Shape Pos (Expr Shape Pos)),
-        pure (add0 fx fy) = Add0 fx fy.
-  Proof.
-    reflexivity.
-  Qed.
-
-  Lemma def_PUSH :
-    forall (fn : Free Shape Pos (Integer Shape Pos)),
-        pure (push fn) = PUSH fn.
-  Proof.
-    reflexivity.
-  Qed.
-
-  Lemma def_ADD :
-        pure (@add Shape Pos) = ADD.
-  Proof.
-    reflexivity.
-  Qed.
-
-End Rewrite_Constructors.
-
-Hint Rewrite -> def_Nil        : smartConstrDB.
-Hint Rewrite <- def_Nil        : invSmartConstrDB.
-Hint Rewrite -> def_Cons       : smartConstrDB.
-Hint Rewrite <- def_Cons       : invSmartConstrDB.
-Hint Rewrite -> def_Code_Nil   : smartConstrDB.
-Hint Rewrite <- def_Code_Nil   : invSmartConstrDB.
-Hint Rewrite -> def_Code_Cons  : smartConstrDB.
-Hint Rewrite <- def_Code_Cons  : invSmartConstrDB.
-Hint Rewrite -> def_Stack_Nil  : smartConstrDB.
-Hint Rewrite <- def_Stack_Nil  : invSmartConstrDB.
-Hint Rewrite -> def_Stack_Cons : smartConstrDB.
-Hint Rewrite <- def_Stack_Cons : invSmartConstrDB.
-Hint Rewrite -> def_Val        : smartConstrDB.
-Hint Rewrite <- def_Val        : invSmartConstrDB.
-Hint Rewrite -> def_Add        : smartConstrDB.
-Hint Rewrite <- def_Add        : invSmartConstrDB.
-Hint Rewrite -> def_PUSH       : smartConstrDB.
-Hint Rewrite <- def_PUSH       : invSmartConstrDB.
-Hint Rewrite -> def_ADD        : smartConstrDB.
-Hint Rewrite <- def_ADD        : invSmartConstrDB.
+  pretty; trivial.
 
 (* Define rules for applying a function to arguments according to its definition. *)
 Section Rewrite_Functions.
@@ -148,7 +53,7 @@ Section Rewrite_Functions.
   Lemma def_append_Nil :
     forall (A : Type)
            (fys : Free Shape Pos (List Shape Pos A)),
-        append (pure nil) fys = fys.
+        append Nil_ fys = fys.
     Proof.
       reflexivity.
     Qed.
@@ -157,30 +62,26 @@ Section Rewrite_Functions.
     forall (A : Type)
            (fx : Free Shape Pos A)
            (fxs fys : Free Shape Pos (List Shape Pos A)),
-        append (pure (cons fx fxs)) fys = pure (cons fx (append fxs fys)).
+        append (Cons_ fx fxs) fys = Cons_ fx (append fxs fys).
     Proof.
       reflexivity.
     Qed.
 
   Lemma def_eval_Val :
     forall (fn : Free Shape Pos (Integer Shape Pos)),
-        eval (pure (val fn))
+        eval (Val_ fn)
         = fn.
-  Proof.
-    reflexivity.
-  Qed.
+  Proof. trivial. Qed.
 
   Lemma def_eval_Add :
     forall (fx fy : Free Shape Pos (Expr Shape Pos)),
-        eval (pure (add0 fx fy))
+        eval (Add0_ fx fy)
         = addInteger (eval fx) (eval fy).
-  Proof.
-    reflexivity.
-  Qed.
+  Proof. trivial. Qed.
 
   Lemma def_exec_Nil :
     forall (stack : Stack Shape Pos),
-        exec Part (pure nil) (pure stack)
+        exec Part Nil_ (pure stack)
         = pure stack.
   Proof.
     destruct stack; reflexivity.
@@ -190,8 +91,8 @@ Section Rewrite_Functions.
     forall (fn : Free Shape Pos (Integer Shape Pos))
            (fcode : Free Shape Pos (Code Shape Pos))
            (stack : Stack Shape Pos),
-        exec Part (pure (cons (pure (push fn)) fcode)) (pure stack)
-        = exec Part fcode (pure (cons fn (pure stack))).
+        exec Part (Cons_ (PUSH_ fn) fcode) (pure stack)
+        = exec Part fcode (Cons_ fn (pure stack)).
   Proof.
     destruct stack; reflexivity.
   Qed.
@@ -200,70 +101,54 @@ Section Rewrite_Functions.
     forall (fcode : Free Shape Pos (Code Shape Pos))
            (fv1 fv2 : Free Shape Pos (Integer Shape Pos))
            (fstack : Free Shape Pos (Stack Shape Pos)),
-        exec Part (pure (cons (pure add) fcode)) (pure (cons fv1 (pure (cons fv2 fstack))))
-        = exec Part fcode (pure (cons (addInteger fv2 fv1) fstack)).
-  Proof.
-    reflexivity.
-  Qed.
+        exec Part (Cons_ ADD_ fcode) (Cons_ fv1 (Cons_ fv2 fstack))
+        = exec Part fcode (Cons_ (addInteger fv2 fv1) fstack).
+  Proof. trivial. Qed.
 
   Lemma def_exec_ADD_0 :
     forall (fcode : Free Shape Pos (Code Shape Pos)),
-        exec Part (pure (cons (pure add) fcode)) (pure nil)
+        exec Part (Cons_ ADD_ fcode) Nil_
         = undefined.
-  Proof.
-    reflexivity.
-  Qed.
+  Proof. trivial. Qed.
 
   Lemma def_exec_ADD_1 :
     forall (fcode : Free Shape Pos (Code Shape Pos))
            (fv1 : Free Shape Pos (Integer Shape Pos)),
-        exec Part (pure (cons (pure add) fcode)) (pure (cons fv1 (pure nil)))
+        exec Part (Cons_ ADD_ fcode) (Cons_ fv1 Nil_)
         = undefined.
-  Proof.
-    reflexivity.
-  Qed.
+  Proof. trivial. Qed.
 
   Lemma def_comp_Val :
     forall (fn : Free Shape Pos (Integer Shape Pos)),
-        comp (pure (val fn))
-        = pure (cons (pure (push fn)) (pure nil)).
-  Proof.
-    reflexivity.
-  Qed.
+        comp (Val_ fn)
+        = Cons_ (PUSH_ fn) Nil_.
+  Proof. trivial. Qed.
 
   Lemma def_comp_Add :
     forall (fx fy : Free Shape Pos (Expr Shape Pos)),
-        comp (pure (add0 fx fy))
-        = append (append (comp fx) (comp fy)) (pure (cons (pure add) (pure nil))).
-  Proof.
-    reflexivity.
-  Qed.
+        comp (Add0_ fx fy)
+        = append (append (comp fx) (comp fy)) (Cons_ ADD_ Nil_).
+  Proof. trivial. Qed.
 
   Lemma def_compApp_Val :
     forall (fn : Free Shape Pos (Integer Shape Pos))
            (fcode : Free Shape Pos (Code Shape Pos)),
-        compApp (pure (val fn)) fcode
-        = pure (cons (pure (push fn)) fcode).
-  Proof.
-    reflexivity.
-  Qed.
+        compApp (Val_ fn) fcode
+        = Cons_ (PUSH_ fn) fcode.
+  Proof. trivial. Qed.
 
   Lemma def_compApp_Add :
     forall (fx fy : Free Shape Pos (Expr Shape Pos))
            (fcode : Free Shape Pos (Code Shape Pos)),
-        compApp (pure (add0 fx fy)) fcode
-        = compApp fx (compApp fy (pure (cons (pure add) fcode))).
-  Proof.
-    reflexivity.
-  Qed.
+        compApp (Add0_ fx fy) fcode
+        = compApp fx (compApp fy (Cons_ ADD_ fcode)).
+  Proof. trivial. Qed.
 
   Lemma def_comp' :
     forall (fexpr : Free Shape Pos (Expr Shape Pos)),
         comp' fexpr
-        = compApp fexpr (pure nil).
-  Proof.
-    reflexivity.
-  Qed.
+        = compApp fexpr Nil_.
+  Proof. trivial. Qed.
 
 End Rewrite_Functions.
 
@@ -296,18 +181,14 @@ Section Rewrite_Functions_Impure.
            (fl2 : Free Shape Pos (List Shape Pos A)),
         append (impure s pf) fl2
         = impure s (fun p => append (pf p) fl2).
-  Proof.
-    reflexivity.
-  Qed.
+  Proof. trivial. Qed.
 
   Lemma def_eval_imp_Expr :
     forall (s : Shape)
            (pf : Pos s -> Free Shape Pos (Expr Shape Pos)),
         eval (impure s pf)
         = impure s (fun p => eval (pf p)).
-  Proof.
-    reflexivity.
-  Qed.
+  Proof. trivial. Qed.
 
   Lemma def_exec_imp_Code :
     forall (s : Shape)
@@ -315,37 +196,31 @@ Section Rewrite_Functions_Impure.
            (fstack : Free Shape Pos (Stack Shape Pos)),
         exec Part (impure s pf) fstack
         = impure s (fun p => exec Part (pf p) fstack).
-  Proof.
-    reflexivity.
-  Qed.
+  Proof. trivial. Qed.
 
   Lemma def_exec_imp_Op :
     forall (s : Shape)
            (pf : Pos s -> Free Shape Pos (Op Shape Pos))
            (fcode : Free Shape Pos (Code Shape Pos))
            (fstack : Free Shape Pos (Stack Shape Pos)),
-        exec Part (pure (cons (impure s pf) fcode)) fstack
-        = impure s (fun p => exec Part (pure (cons (pf p) fcode)) fstack).
-  Proof.
-    reflexivity.
-  Qed.
+        exec Part (Cons_ (impure s pf) fcode) fstack
+        = impure s (fun p => exec Part (Cons_ (pf p) fcode) fstack).
+  Proof. trivial. Qed.
 
   Lemma def_exec_Nil_imp_Stack :
     forall (s : Shape)
            (pf : Pos s -> Free Shape Pos (Stack Shape Pos)),
-        exec Part (pure nil) (impure s pf)
-        = impure s (fun p => exec Part (pure nil) (pf p)).
-  Proof.
-    reflexivity.
-  Qed.
+        exec Part Nil_ (impure s pf)
+        = impure s (fun p => exec Part Nil_ (pf p)).
+  Proof. trivial. Qed.
 
   Lemma def_exec_Op_imp_Stack :
     forall (op : Op Shape Pos)
            (fcode : Free Shape Pos (Code Shape Pos))
            (s : Shape)
            (pf : Pos s -> Free Shape Pos (Stack Shape Pos)),
-        exec Part (pure (cons (pure op) fcode)) (impure s pf)
-        = impure s (fun p => exec Part (pure (cons (pure op) fcode)) (pf p)).
+        exec Part (Cons_ (pure op) fcode) (impure s pf)
+        = impure s (fun p => exec Part (Cons_ (pure op) fcode) (pf p)).
   Proof.
     destruct op; reflexivity.
   Qed.
@@ -355,20 +230,16 @@ Section Rewrite_Functions_Impure.
            (s : Shape)
            (fv1 : Free Shape Pos (Integer Shape Pos))
            (pf : Pos s -> Free Shape Pos (Stack Shape Pos)),
-        exec Part (pure (cons (pure add) fcode)) (pure (cons fv1 (impure s pf)))
-        = impure s (fun p => exec Part (pure (cons (pure add) fcode)) (pure (cons fv1 (pf p)))).
-  Proof.
-    reflexivity.
-  Qed.
+        exec Part (Cons_ ADD_ fcode) (Cons_ fv1 (impure s pf))
+        = impure s (fun p => exec Part (Cons_ ADD_ fcode) (Cons_ fv1 (pf p))).
+  Proof. trivial. Qed.
 
   Lemma def_comp_imp_Expr :
     forall (s : Shape)
            (pf : Pos s -> Free Shape Pos (Expr Shape Pos)),
         comp (impure s pf)
         = impure s (fun p => comp (pf p)).
-  Proof.
-    reflexivity.
-  Qed.
+  Proof. trivial. Qed.
 
   Lemma def_compApp_imp_Expr :
     forall (s : Shape)
@@ -376,18 +247,14 @@ Section Rewrite_Functions_Impure.
            (fcode : Free Shape Pos (Code Shape Pos)),
         compApp (impure s pf) fcode
         = impure s (fun p => compApp (pf p) fcode).
-  Proof.
-    reflexivity.
-  Qed.
+  Proof. trivial. Qed.
 
   Lemma def_comp'_imp_Expr :
     forall (s : Shape)
            (pf : Pos s -> Free Shape Pos (Expr Shape Pos)),
         comp' (impure s pf)
         = impure s (fun p => comp' (pf p)).
-  Proof.
-    reflexivity.
-  Qed.
+  Proof. trivial. Qed.
 
 End Rewrite_Functions_Impure.
 
@@ -414,9 +281,7 @@ Section Rewrite_Helper_Functions.
            (fl1 fl2 : Free Shape Pos (List Shape Pos A)),
         append0 Shape Pos A fl2 fl1
         = append fl1 fl2.
-  Proof.
-    reflexivity.
-  Qed.
+  Proof. trivial. Qed.
 
   Lemma def_append1 :
     forall (A : Type)
@@ -424,43 +289,33 @@ Section Rewrite_Helper_Functions.
            (fl2 : Free Shape Pos (List Shape Pos A)),
         append1 Shape Pos A fl2 l1
         = append (pure l1) fl2.
-  Proof.
-    reflexivity.
-  Qed.
+  Proof. trivial. Qed.
 
   Lemma def_eval0 :
     forall (expr : Expr Shape Pos),
         eval0 Shape Pos expr
         = eval (pure expr).
-  Proof.
-    reflexivity.
-  Qed.
+  Proof. trivial. Qed.
 
   Lemma def_exec0 :
     forall (code : Code Shape Pos)
            (fstack : Free Shape Pos (Stack Shape Pos)),
         exec0 Shape Pos Part code fstack
         = exec Part (pure code) fstack.
-  Proof.
-    reflexivity.
-  Qed.
+  Proof. trivial. Qed.
 
   Lemma def_comp0 :
     forall (expr : Expr Shape Pos),
         comp0 Shape Pos expr
         = comp (pure expr).
-  Proof.
-    reflexivity.
-  Qed.
+  Proof. trivial. Qed.
 
   Lemma def_compApp0 :
     forall (expr : Expr Shape Pos)
            (fcode : Free Shape Pos (Code Shape Pos)),
         compApp0 Shape Pos expr fcode
         = compApp (pure expr) fcode.
-  Proof.
-    reflexivity.
-  Qed.
+  Proof. trivial. Qed.
 
 End Rewrite_Helper_Functions.
 
@@ -473,26 +328,24 @@ Hint Rewrite def_compApp0 : prettyDB.
 
 (* Define specific rules for the [Maybe] monad. *)
 Section Rewrite_Maybe.
-
-  Definition Shape := Maybe.Shape.
-  Definition Pos   := Maybe.Pos.
-  Definition Part  := Maybe.Partial.
+  Variable Shape  : Type.
+  Variable Pos    : Shape -> Type.
+  Variable Inj    : Injectable Maybe.Shape Maybe.Pos Shape Pos.
+  Definition Part := Maybe.Partial Shape Pos.
 
   (* Smart constructors. *)
   Lemma def_Just :
     forall (A : Type)
            (x : A),
         pure x = Just x.
-  Proof.
-    reflexivity.
-  Qed.
+  Proof. trivial. Qed.
 
   Lemma def_Nothing :
     forall (A : Type),
-        impure tt (fun (p : Pos tt) => match p with end) = @Nothing A.
-  Proof.
-    reflexivity.
-  Qed.
+        impure (injS tt) (fun p : Pos (injS tt) =>
+      match (injP p) : Void.Void with end)
+      = @Nothing _ _ _ A.
+  Proof. trivial. Qed.
 
   (* As this monad has only one impure case, we can generalize [def_Nothing]. *)
   Lemma impure_Nothing :
@@ -511,23 +364,20 @@ Section Rewrite_Maybe.
   Lemma def_undefined_Maybe :
     forall (A : Type),
       @undefined Shape Pos Part A = Nothing.
-  Proof.
-    reflexivity.
-  Qed.
+  Proof. trivial. Qed.
 
   Lemma def_error_Maybe :
-  forall (A : Type) (err : string),
+    forall (A : Type)
+           (err : string),
     @error Shape Pos Part A err = Nothing.
-  Proof.
-    reflexivity.
-  Qed.
+  Proof. trivial. Qed.
 
 End Rewrite_Maybe.
 
 (* We won't use the smart constructor [Just] as it interferes with other smart constructors. *)
 (* Hint Rewrite -> def_Just         : smartConstrDB. *)
-Hint Rewrite <- def_Just         : invSmartConstrDB.
-Hint Rewrite -> impure_Nothing   : smartConstrDB.
-Hint Rewrite <- def_Nothing      : invSmartConstrDB.
+Hint Rewrite <- def_Just         : simplDB.
+Hint Rewrite -> impure_Nothing   : prettyDB.
+Hint Rewrite <- def_Nothing      : simplDB.
 Hint Rewrite def_undefined_Maybe : simplDB prettyDB.
 Hint Rewrite def_error_Maybe     : simplDB prettyDB.
